Update liveness for mutual recursion.

Liveness.v
@@ -1,4 +1,4 @@
-Require Import AllInRel List Map Env DecSolve.
+Require Import AllInRel List Map Env DecSolve InRel.
 Require Import IL Annotation AutoIndTac Bisim Exp MoreExp Filter Rename.
 
 Set Implicit Arguments.
@@ -27,6 +27,11 @@ Definition isImperative (o:overapproximation) :=
   end.
 
 (** ** Inductive Definition of Liveness *)
+
+
+Definition mkLv (alL:list (ann (set var))) (F:list (params*stmt)) :=
+  zip (fun als f => (getAnn  als,fst f)) alL F.
+
 
 Inductive live_sound (i:overapproximation) : list (set var*params) -> stmt -> ann (set var) -> Prop :=
 | LOpr x Lv b lv e (al:ann (set var))
@@ -57,13 +62,18 @@ Inductive live_sound (i:overapproximation) : list (set var*params) -> stmt -> an
   -> (getAnn al\{{x}}) ⊆ lv
   -> x ∈ getAnn al
   -> live_sound i Lv (stmtExtern x f Y b) (ann1 lv al)
-| LLet Lv s Z b lv als alb
-  : live_sound i ((getAnn als,Z)::Lv) s als
-  -> live_sound i ((getAnn als,Z)::Lv) b alb
-  -> (of_list Z) ⊆ getAnn als  (** Functional Liveness requires the globals of a function to be live at the definition (for building the closure) *)
-  -> (if isFunctional i then (getAnn als \ of_list Z ⊆ lv) else True)
+| LLet Lv Zs b lv als alb
+  : live_sound i (mkLv als Zs++Lv) b alb
+    -> length Zs = length als
+  -> (forall n Zs' a, get Zs n Zs' ->
+                     get als n a ->
+                     live_sound i (mkLv als Zs ++ Lv) (snd Zs') a)
+  -> (forall n Zs' a, get Zs n Zs' ->
+                  get als n a ->
+                  (of_list (fst Zs')) ⊆ getAnn a
+                  /\ (if isFunctional i then (getAnn a \ of_list (fst Zs')) ⊆ lv else True))
   -> getAnn alb ⊆ lv
-  -> live_sound i Lv (stmtFun Z s b)(ann2 lv als alb).
+  -> live_sound i Lv (stmtFun Zs b)(annF lv als alb).
 
 
 (** ** Relation between different overapproximations *)
@@ -72,6 +82,7 @@ Lemma live_sound_overapproximation_I Lv s slv
 : live_sound FunctionalAndImperative Lv s slv -> live_sound Imperative Lv s slv.
 Proof.
   intros. general induction H; simpl in * |- *; econstructor; simpl; eauto.
+  - intros. edestruct H3; eauto.
 Qed.
 
 Lemma live_sound_overapproximation_F Lv s slv
@@ -110,9 +121,7 @@ Proof.
     destruct if; simpl in *; eauto; dcr; subst.
     rewrite <- H0. rewrite <- H4. reflexivity.
     cset_tac; intuition; eauto.
-  - econstructor; eauto 20 using PIR2.
-    eapply IHlive_sound1. econstructor; intuition.
-    eapply IHlive_sound2. econstructor; intuition.
+  - econstructor; eauto 20 using PIR2_app.
 Qed.
 
 Lemma live_sound_monotone2 i LV s lv a
@@ -129,7 +138,8 @@ Proof.
   - econstructor; eauto using live_exp_sound_incl; etransitivity; eauto.
   - econstructor; eauto using live_exp_sound_incl.
     etransitivity; eauto.
-  - econstructor; eauto. destruct i; simpl; eauto; cset_tac; intuition.
+  - econstructor; eauto. intros. edestruct H3; eauto.
+    destruct i; simpl; eauto; cset_tac; intuition.
     cset_tac; intuition.
 Qed.
 
@@ -153,8 +163,11 @@ Proof.
     edestruct map_get_4; eauto; dcr; subst.
     exploit Exp.freeVars_live; eauto.
   + eapply union_subset_3.
-    rewrite IHlive_sound1; eauto.
-    rewrite IHlive_sound2; eauto.
+    eapply list_union_incl; intros; eauto.
+    inv_map H5. edestruct (get_length_eq _ H6 H0); eauto.
+    edestruct H3; eauto. simpl in *. exploit H2; eauto.
+    rewrite X; eauto.
+    rewrite IHlive_sound; eauto.
 Qed.
 
 (** ** Liveness is stable under renaming *)
@@ -163,7 +176,25 @@ Definition live_rename_L_entry (ϱ:env var) (x:set var * params)
  := (lookup_set ϱ (fst x), lookup_list ϱ (snd x)).
 
 Definition live_rename_L (ϱ:env var) DL
- := List.map (live_rename_L_entry ϱ) DL.
+  := List.map (live_rename_L_entry ϱ) DL.
+
+Lemma live_rename_L_mkLv ϱ als Zs
+: length Zs = length als
+  -> (live_rename_L ϱ (mkLv als Zs) =
+     mkLv (List.map (mapAnn (lookup_set ϱ)) als)
+          (List.map
+             (fun Zs0 : params * stmt =>
+                (lookup_list ϱ (fst Zs0), rename ϱ (snd Zs0))) Zs)).
+Proof.
+  intros. length_equify. general induction H; simpl; eauto.
+  - f_equal; eauto. rewrite getAnn_mapAnn; reflexivity.
+Qed.
+
+Lemma live_rename_L_app ϱ L L'
+: live_rename_L ϱ (L ++ L') = live_rename_L ϱ L ++ live_rename_L ϱ L'.
+Proof.
+  unfold live_rename_L. rewrite map_app; reflexivity.
+Qed.
 
 Lemma live_rename_sound i DL s an (ϱ:env var)
 : live_sound i DL s an
@@ -203,23 +234,51 @@ Proof.
       eapply lookup_set_incl; eauto.
     + rewrite getAnn_mapAnn; eauto. eapply lookup_set_spec; eauto.
   - econstructor; eauto; try rewrite getAnn_mapAnn; eauto.
-    eapply IHlive_sound1. eapply IHlive_sound2.
-    rewrite of_list_lookup_list; eauto. eapply lookup_set_incl; eauto.
-    destruct if; eauto.
-    rewrite of_list_lookup_list; eauto.
-    rewrite lookup_set_minus_incl; eauto.
-    destruct i; simpl; eauto; eapply lookup_set_incl; eauto.
-    eapply lookup_set_incl; eauto.
+    + rewrite <- live_rename_L_mkLv, <- live_rename_L_app; eauto.
+    + repeat rewrite map_length; eauto.
+    + intros. inv_map H5. inv_map H6.
+      rewrite <- live_rename_L_mkLv, <- live_rename_L_app; eauto.
+      eapply H2; eauto.
+    + intros. inv_map H6; inv_map H5.
+      exploit H3; eauto. simpl. split.
+      rewrite of_list_lookup_list; eauto.
+      rewrite getAnn_mapAnn. dcr.
+      eapply lookup_set_incl; eauto.
+      destruct if; eauto.
+      rewrite getAnn_mapAnn. dcr.
+      rewrite of_list_lookup_list; eauto.
+      rewrite lookup_set_minus_incl; eauto.
+      eapply lookup_set_incl; eauto.
+    + eapply lookup_set_incl; eauto.
 Qed.
 
 (** ** For functional programs, only free variables are significant *)
 
 Inductive approxF :  F.block -> F.block -> Prop :=
- | approxFI E E' Z s
+ | approxFI E E' Z s n
     : agree_on eq (IL.freeVars s \ of_list Z) E E'
-    ->  approxF (F.blockI E Z s) (F.blockI E' Z s).
+    ->  approxF (F.blockI E Z s n) (F.blockI E' Z s n).
 
 Unset Printing Records.
+
+Lemma mkBlocks_approxF s0 E E' s i
+: agree_on eq (list_union
+                 (List.map
+                    (fun f : params * stmt =>
+                       IL.freeVars (snd f) \ of_list (fst f)) s) ++
+                     IL.freeVars s0) E E'
+  -> PIR2 approxF (mapi_impl (F.mkBlock E) i s) (mapi_impl (F.mkBlock E') i s).
+Proof.
+  intros.
+  general induction s; eauto using PIR2. simpl.
+  - econstructor. econstructor.
+    eapply agree_on_incl; eauto.
+    rewrite <- get_list_union_map; eauto using get.
+    eapply IHs.
+    eapply agree_on_incl; eauto. simpl.
+    rewrite <- SetOperations.list_union_cons. reflexivity.
+Qed.
+
 
 Inductive freeVarSimF : F.state -> F.state -> Prop :=
   freeVarSimFI (E E':onv val) L L' s
@@ -253,6 +312,7 @@ Proof.
     + exploit omap_exp_eval_agree; eauto.
       one_step.
       simpl. eapply freeVarSimF_sim. econstructor; eauto.
+      eapply PIR2_drop; eauto.
       eapply update_with_list_agree; eauto.
       exploit omap_length; eauto. rewrite map_length; congruence.
     + exploit omap_exp_eval_agree; eauto.
@@ -283,18 +343,17 @@ Proof.
       eapply agree_on_incl; eauto. congruence.
   - one_step.
     eapply freeVarSimF_sim; econstructor; eauto.
-    econstructor; eauto using agree_on_incl.
-    econstructor; eauto using agree_on_incl.
+    eapply PIR2_app; eauto. eapply mkBlocks_approxF; eauto.
     eapply agree_on_incl; eauto.
 Qed.
 
 (** ** Since live variables contain free variables, liveness contains all variables significant to an IL/F program *)
 
 Inductive approxF' : list (set var * params) -> F.block -> F.block -> Prop :=
-  approxFI' DL E E' Z s lv
+  approxFI' DL E E' Z s lv n
   : live_sound Functional ((getAnn lv, Z)::DL) s lv
     -> agree_on eq (getAnn lv \ of_list Z) E E'
-    ->  approxF' ((getAnn lv,Z)::DL) (F.blockI E Z s) (F.blockI E' Z s).
+    ->  approxF' ((getAnn lv,Z)::DL) (F.blockI E Z s n) (F.blockI E' Z s n).
 
 Inductive liveSimF : F.state -> F.state -> Prop :=
   liveSimFI (E E':onv val) L L' s Lv lv
@@ -320,17 +379,34 @@ Qed.
 (** ** Live variables contain all variables significant to an IL/I program *)
 
 Inductive approxI
-  : list (set var * params) -> I.block -> I.block -> Prop :=
-  approxII DL Z s lv
-  : live_sound Imperative ((getAnn lv, Z)::DL) s lv
-    ->  approxI ((getAnn lv,Z)::DL) (I.blockI Z s) (I.blockI Z s).
+  : list (set var * params) -> set var * params -> I.block -> I.block -> Prop :=
+  approxII DL Z s lv n
+  : live_sound Imperative DL s lv
+    ->  approxI DL (getAnn lv,Z) (I.blockI Z s n) (I.blockI Z s n).
 
 Inductive liveSimI : I.state -> I.state -> Prop :=
   liveSimII (E E':onv val) L s Lv lv
   (LS:live_sound Imperative Lv s lv)
-  (LA:AIR3 approxI Lv L L)
+  (LA:inRel approxI Lv L L)
   (AG:agree_on eq (getAnn lv) E E')
   : liveSimI (L, E, s) (L, E', s).
+
+Lemma approx_mutual_block alF F Lv i
+:
+  length alF = length F
+  ->  (forall (n : nat) Zs (als : ann (set var)),
+        get F n Zs ->
+        get alF n als -> live_sound Imperative Lv (snd Zs) als)
+  -> mutual_block (approxI Lv) i (mkLv alF F) (mapi_impl I.mkBlock i F) (mapi_impl I.mkBlock i F).
+Proof.
+  unfold I.mkBlocks, mkLv, mapi.
+  intros. length_equify.
+  general induction H; simpl.
+  - econstructor.
+  - econstructor; eauto.
+    + eapply IHlength_eq; intros; eauto using get.
+    + destruct y. eauto using approxI, get.
+Qed.
 
 Lemma liveSimI_sim σ1 σ2
   : liveSimI σ1 σ2 -> bisim σ1 σ2.
@@ -353,11 +429,12 @@ Proof.
     eapply liveSimI_sim; econstructor; eauto using agree_on_incl.
     exploit exp_eval_live_agree; eauto.
     no_step.
-  - provide_invariants_3.
+  - inRel_invs.
     case_eq (omap (exp_eval E) Y); intros.
     + exploit omap_exp_eval_live_agree; eauto.
       one_step; simpl; try congruence.
       simpl. eapply liveSimI_sim. econstructor; eauto.
+      eapply (inRel_drop LA H3).
       eapply update_with_list_agree; eauto using agree_on_incl.
       exploit omap_length; eauto. rewrite map_length. congruence.
     + exploit omap_exp_eval_live_agree; eauto.
@@ -381,9 +458,9 @@ Proof.
     + no_step.
   - one_step.
     eapply liveSimI_sim; econstructor; eauto.
-    econstructor; eauto using agree_on_incl.
-    econstructor; eauto using agree_on_incl.
-    eapply agree_on_incl; eauto.
+    + econstructor; eauto using agree_on_incl.
+      eapply approx_mutual_block; eauto.
+    + eapply agree_on_incl; eauto.
 Qed.
 
 (*
